theories/simulations/ctxrefine/CtxRefine.v
@@ -4,7 +4,7 @@ Require Import LMod Mod.
 Require Import allocs.
 From iris.proofmode Require Import proofmode.
 
-Definition refines_lmod (ms_src ms_tgt: LMod.t) : Prop :=
+Definition refines_lmod (ms_tgt ms_src: LMod.t) : Prop :=
   Beh.of_itree (LMod.compile ms_tgt tt↑) <1=
   Beh.of_itree (LMod.compile ms_src tt↑).
 
@@ -12,7 +12,7 @@ Section CTX_REFINE.
   Context `{!crisG Γ Σ α β τ _S _I}.
 
   (* Definition of ctx refinement in Mod Level. *)
-  Definition refines (mps : Mod.modc) (mpt : Mod.modc) : Prop :=
+  Definition refines (mpt : Mod.modc) (mps : Mod.modc) : Prop :=
     let ms := mps.1 in let Ps := mps.2 in
     let mt := mpt.1 in let Pt := mpt.2 in
 
@@ -23,12 +23,13 @@ Section CTX_REFINE.
         ∃ rt,
           ✓ rt /\ (Own rt ⊢ |==> winv (∅,∅) ∗ Pt)%I /\
           refines_lmod
-            (Mod.to_lmod ms rs)
-            (Mod.to_lmod mt rt).
+            (Mod.to_lmod mt rt)
+            (Mod.to_lmod ms rs).
 
-  Definition ctx_refines (mps mpt : Mod.modc) : Prop :=
+  Definition ctx_refines (mpt mps: Mod.modc) : Prop :=
     ∀ (ctx : Mod.modc),
-      refines (mps.1 ★ ctx.1, mps.2 ∗ ctx.2)%I
-              (mpt.1 ★ ctx.1, mpt.2 ∗ ctx.2)%I.
+      refines
+        (mpt.1 ★ ctx.1, mpt.2 ∗ ctx.2)%I
+        (mps.1 ★ ctx.1, mps.2 ∗ ctx.2)%I.
 End CTX_REFINE.
 Global Instance: Params (@ctx_refines) 1 := {}.
