helping/HelpingFacts.v
@@ -26,26 +26,26 @@ Section Helping.
     {jobID retID : Type} (jobs : jobID -> _) (sp : specmap)
     (REF1: ∀ Q mn,
       refines
-        (mM mn ★ CFilter.filter (Helping.exports mn ∪ fns) (SchI.t ★ ctx) ★ (HelpingOn.t (retID:=retID) mn jobs sp), (P1 ∗ Q)%I)
-        (CFilter.filter (Helping.exports mn) mI ★ CFilter.filter (Helping.exports mn ∪ fns) (SchI.t ★ ctx) ★ (HelpingDummy.t mn), Q))
+        (CFilter.filter (Helping.exports mn) mI ★ CFilter.filter (Helping.exports mn ∪ fns) (SchI.t ★ ctx) ★ (HelpingDummy.t mn), Q)
+        (mM mn ★ CFilter.filter (Helping.exports mn ∪ fns) (SchI.t ★ ctx) ★ (HelpingOn.t (retID:=retID) mn jobs sp), (P1 ∗ Q)%I))
     (REF2: ∀ Q mn,
       refines
-        (mA ★ CFilter.filter (Helping.exports mn ∪ fns) (SchI.t ★ ctx), (P2 ∗ Q)%I)
-        (mM mn ★ CFilter.filter (Helping.exports mn ∪ fns) (SchI.t ★ ctx) ★ HelpingOff.t mn jobs sp, Q))
+        (mM mn ★ CFilter.filter (Helping.exports mn ∪ fns) (SchI.t ★ ctx) ★ HelpingOff.t mn jobs sp, Q)
+        (mA ★ CFilter.filter (Helping.exports mn ∪ fns) (SchI.t ★ ctx), (P2 ∗ Q)%I))
     (DISJ: get_fids (dom (Mod.fnsems (mA ★ SchI.t ★ ctx))) ## fns)
     :
     refines
-      (mA ★ SchI.t ★ ctx, (P1 ∗ P2 ∗ P)%I)
-      (mI ★ CFilter.filter fns (SchI.t ★ ctx), P).
+      (mI ★ CFilter.filter fns (SchI.t ★ ctx), P)
+      (mA ★ SchI.t ★ ctx, (P1 ∗ P2 ∗ P)%I).
   Proof using.
     set (mn := mname_long (S (max
                  (maxlen (elements (get_fids (dom (Mod.fnsems (mA ★ mI ★ SchI.t ★ ctx))))))
                  (maxlen (Mod.scopes (mA ★ mI ★ SchI.t ★ ctx)))))).
 
-    etrans; cycle 1.
+    etrans.
     { eapply ctxr_refines, (CFilter.intro_filter (Helping.exports mn)). }
 
-    etrans; cycle 1.
+    etrans.
     { eapply CFilter.intro_module with (mask := Helping.exports mn) (mc := (HelpingDummy.t mn)); et.
       { eapply helping_dummy_wf. }
       { intros ? a ->%elem_of_list_singleton. subst mn. eapply elem_of_maxlen in a.
@@ -64,28 +64,28 @@ Section Helping.
       { set_solver+. }
     }
 
-    etrans; cycle 1.
+    etrans.
     { rewrite CFilter.filter_app -CFilter.filter_union -!assoc. apply REF1. }
 
-    etrans; cycle 1.
+    etrans.
     { eapply ctxr_refines.
       rewrite CFilter.filter_app.
       ctxr_drop. ctxr_rotate. ctxr_drop.
       eapply helping_onoff_correct; et. set_solver.
     }
 
-    etrans; cycle 1.
-    { evar_at_last_1; [apply REF2|].
-      rewrite !CFilter.filter_app -!assoc. do 2 f_equal.
+    etrans.
+    { evar_at_last_2; [apply REF2|]. 
+      do 2 f_equal. rewrite !CFilter.filter_app -!assoc.
       rewrite (comm _ (_ _ SchI.t)) assoc. refl.
     }
 
-    etrans; cycle 1.
+    etrans.
     { eapply ctxr_refines.
       ctxr_rotate. ctxr_drop. eapply CFilter.intro_filter.
     }
     repeat erewrite <-CFilter.filter_app. rewrite (comm _ _ mA).
-    etrans; cycle 1.
+    etrans.
     { eapply CFilter.elim_filter.
       rewrite disjoint_union_r. split; et.
       intros i Hi1 Hi2. rewrite -elem_of_elements in Hi1; eapply elem_of_maxlen in Hi1.
@@ -102,38 +102,27 @@ Section Helping.
       {jobID retID : Type} (jobs : jobID -> _) (sp : specmap) :
     (∀ mn,
       ctx_refines
-        (mM mn ★ CFilter.filter (Helping.exports mn) (mE ★ SchI.t) ★ (HelpingOn.t (retID:=retID) mn jobs sp), P1)
-        (CFilter.filter (Helping.exports mn) (mI ★ mE ★ SchI.t) ★ (HelpingDummy.t mn), emp%I)) →
+        (CFilter.filter (Helping.exports mn) (mI ★ mE ★ SchI.t) ★ (HelpingDummy.t mn), emp%I)
+        (mM mn ★ CFilter.filter (Helping.exports mn) (mE ★ SchI.t) ★ (HelpingOn.t (retID:=retID) mn jobs sp), P1)) →
     (∀ mn,
       (ctx_refines
-        (mA    ★ CFilter.filter (Helping.exports mn) (mE ★ SchI.t), P2)
-        (mM mn ★ CFilter.filter (Helping.exports mn) (mE ★ SchI.t) ★ HelpingOff.t mn jobs sp, emp%I))) →
+        (mM mn ★ CFilter.filter (Helping.exports mn) (mE ★ SchI.t) ★ HelpingOff.t mn jobs sp, emp%I))
+        (mA    ★ CFilter.filter (Helping.exports mn) (mE ★ SchI.t), P2)) →
     ctx_refines
-      (mA ★ mE ★ SchI.t, (P1 ∗ P2)%I)
-      (mI ★ mE ★ SchI.t, emp%I).
+      (mI ★ mE ★ SchI.t, emp%I)
+      (mA ★ mE ★ SchI.t, (P1 ∗ P2)%I).
   Proof.
     intros REF1 REF2 [ctx P]; s.
     rewrite (comm _ mE) -!assoc.
-    etrans; [eapply helping_refines with (mI := mI) (mM := mM) (fns:=∅)|]; i.
-    - rewrite CFilter.filter_union CFilter.filter_empty -{2}(left_id _ bi_sep Q).
+    etrans; [|eapply helping_refines with (mI := mI) (mM := mM) (fns:=∅)]; cycle 1; i.
+    - rewrite CFilter.filter_union CFilter.filter_empty -{1}(left_id _ bi_sep Q).
       evar_at_last_1; [evar_at_last_2|]; [eapply (REF1 _ (_,_))|..]; s.
-      + rewrite !CFilter.filter_app -!assoc.
-        do 2 f_equal. symmetry. rewrite (comm _ (_ _ SchI.t)) -!assoc. f_equal.
-        rewrite !assoc (comm _ _ (_ _ SchI.t)) -!assoc. f_equal.
-        rewrite (comm _ (_ _ ctx)). et.
-      + rewrite !CFilter.filter_app -!assoc.
-        do 2 f_equal. symmetry. rewrite (comm _ (_ _ SchI.t)) -!assoc. f_equal.
-        rewrite !assoc (comm _ _ (_ _ SchI.t)) -!assoc. f_equal.
-        rewrite (comm _ (_ _ ctx)). et.
-    - rewrite CFilter.filter_union CFilter.filter_empty -{2}(left_id _ bi_sep Q).
+      + f_equal. rewrite !CFilter.filter_app. instantiate (1:= _ _ ctx). mod_eq_solver.
+      + f_equal. rewrite !CFilter.filter_app. mod_eq_solver.
+    - rewrite CFilter.filter_union CFilter.filter_empty -{1}(left_id _ bi_sep Q).
       evar_at_last_1; [evar_at_last_2|]; [eapply (REF2 _ (_,_))|..]; s.
-      + rewrite !CFilter.filter_app -!assoc.
-        do 2 f_equal. symmetry. rewrite (comm _ (_ _ SchI.t)) -!assoc. f_equal.
-        rewrite (comm _ (_ _ ctx)). et.
-      + rewrite !CFilter.filter_app -!assoc.
-        do 2 f_equal. symmetry. rewrite (comm _ (_ _ SchI.t)) -!assoc. f_equal.
-        rewrite !assoc (comm _ _ (_ _ SchI.t)) -!assoc. f_equal.
-        rewrite (comm _ (_ _ ctx)). et.
+      + f_equal. rewrite !CFilter.filter_app. instantiate (1:= _ _ ctx). mod_eq_solver.
+      + f_equal. rewrite !CFilter.filter_app. mod_eq_solver.
     - apply disjoint_empty_r.
     - rewrite CFilter.filter_empty left_id. refl.
   Qed.
