prophecy/ProphecyFacts.v
@@ -17,24 +17,25 @@ Section prophecy.
   Lemma prophecy_refines sz (mds mdt ctx : Mod.t) (mdm : string → Mod.t) (Pm Ps : iProp Σ)
     (REF1: ∀ Q,
       refines
-        (mdm (mname_long sz) ★ ProphecyI.t (mname_long sz) ★ CFilter.filter (Prophecy.exports (mname_long sz)) ctx, (Pm ∗ Q)%I)
-        (CFilter.filter (Prophecy.exports (mname_long sz)) mdt ★ ProphecyI.t (mname_long sz) ★ CFilter.filter (Prophecy.exports (mname_long sz)) ctx, Q))
+        (CFilter.filter (Prophecy.exports (mname_long sz)) mdt ★ ProphecyI.t (mname_long sz) ★ CFilter.filter (Prophecy.exports (mname_long sz)) ctx, Q)
+        (mdm (mname_long sz) ★ ProphecyI.t (mname_long sz) ★ CFilter.filter (Prophecy.exports (mname_long sz)) ctx, (Pm ∗ Q)%I))
     (REF2: ∀ Q,
       refines
-        (mds ★ CFilter.filter (Prophecy.exports (mname_long sz)) ctx, (Ps ∗ Q)%I)
-        (mdm (mname_long sz) ★ ProphecyA.t (mname_long sz) ∅ ★ CFilter.filter (Prophecy.exports (mname_long sz)) ctx, Q))
+        (mdm (mname_long sz) ★ ProphecyA.t (mname_long sz) ∅ ★ CFilter.filter (Prophecy.exports (mname_long sz)) ctx, Q)
+        (mds ★ CFilter.filter (Prophecy.exports (mname_long sz)) ctx, (Ps ∗ Q)%I))
     (SZ: sz > max (maxlen (elements (get_fids (dom (Mod.fnsems (mds ★ mdt ★ ctx))))))
                   (maxlen (Mod.scopes (mds ★ mdt ★ ctx))))
     (Realmdm: real_mod (mdm (mname_long sz)))
     (Realctx: real_mod ctx)
     :
-    refines (mds ★ ctx, Pm ∗ ProphecyA.initial_cond ∗ Ps)%I
-            (mdt ★ ctx, emp%I).
+    refines
+      (mdt ★ ctx, emp%I)
+      (mds ★ ctx, Pm ∗ ProphecyA.initial_cond ∗ Ps)%I.
   Proof.
-    etrans; cycle 1.
+    etrans.
     { eapply ctxr_refines, (CFilter.intro_filter (Prophecy.exports (mname_long sz))). }
 
-    etrans; cycle 1.
+    etrans.
     { eapply CFilter.intro_module with (mc := ProphecyI.t (mname_long sz)).
       { econs; [mod_tac|prove_nodup]. }
       { set_solver. }
@@ -46,20 +47,20 @@ Section prophecy.
       { set_solver+. }
     }
     rewrite CFilter.filter_app.
-    etrans; cycle 1.
+    etrans.
     { rewrite -assoc (comm _ _ (ProphecyI.t _)). apply REF1. }
-    etrans; cycle 1.
+    etrans.
     { rewrite (comm _ (ProphecyI.t _)) assoc.
       eapply ProphIA.adequacy_refines; eauto.
       eapply real_mod_add; eauto using CFilter.real_mod.
     }
-    etrans; cycle 1.
+    etrans.
     { rewrite -assoc (comm _ _ (ProphecyA.t _ _)). apply REF2. }
-    etrans; cycle 1.
+    etrans.
     { eapply ctxr_refines. ctxr_rotate. ctxr_drop.
       eapply CFilter.intro_filter. }
     erewrite <-!CFilter.filter_app. ctxr_norm.
-    etrans; cycle 1.
+    etrans.
     { eapply CFilter.elim_filter.
       intros i Hi1 Hi2; rewrite -elem_of_elements in Hi1; eapply elem_of_maxlen in Hi1.
       rewrite Mod.dom_fnsems_add maxlen_get_fids_union in Hi1.
@@ -74,24 +75,24 @@ Section prophecy.
   Lemma prophecy_main (mds mdt ctx : Mod.t) (mdm : string → Mod.t) (Pm Ps : iProp Σ) :
     (∀ mn,
       ctx_refines
-        (mdm mn ★ ProphecyI.t mn, Pm)
-        (CFilter.filter (Prophecy.exports mn) mdt ★ ProphecyI.t mn, emp%I)) →
+        (CFilter.filter (Prophecy.exports mn) mdt ★ ProphecyI.t mn, emp%I)
+        (mdm mn ★ ProphecyI.t mn, Pm)) →
     (∀ mn,
       ctx_refines
-        (mds, Ps)
-        (mdm mn ★ ProphecyA.t mn ∅, emp%I)) →
+        (mdm mn ★ ProphecyA.t mn ∅, emp%I)
+        (mds, Ps)) →
     (∀ mn, real_mod (mdm mn)) →
     real_mod ctx →
-    refines (mds ★ ctx, Pm ∗ ProphecyA.initial_cond ∗ Ps)%I (mdt ★ ctx, emp%I).
+    refines (mdt ★ ctx, emp%I) (mds ★ ctx, Pm ∗ ProphecyA.initial_cond ∗ Ps)%I.
   Proof.
     intros REF1 REF2 Rmdm Rctx; s.
     set (sz := S (max
                  (maxlen (elements (get_fids (dom (Mod.fnsems (mds ★ mdt ★ ctx))))))
                  (maxlen (Mod.scopes (mds ★ mdt ★ ctx))))).
     eapply prophecy_refines with (sz:=sz); i; eauto using prophecy_exports_long; try nia.
-    - eapply ctxr_refines. rewrite !assoc -{2}(left_id _ bi_sep Q).
+    - eapply ctxr_refines. rewrite !assoc -{1}(left_id _ bi_sep Q).
       eapply ctxr_frameR, ctxr_cond_frameR. eapply REF1.
-    - eapply ctxr_refines. rewrite !assoc -{2}(left_id _ bi_sep Q).
+    - eapply ctxr_refines. rewrite !assoc -{1}(left_id _ bi_sep Q).
       eapply ctxr_frameR, ctxr_cond_frameR. eapply REF2.
   Qed.
 
